examples/ghc/lib/CoreSubst.v
@@ -27,6 +27,7 @@ Require GHC.Err.
 Require GHC.List.
 Require GHC.Num.
 Require Id.
+Require Maybes.
 Require Name.
 Require Panic.
 Require UniqSupply.
@@ -55,27 +56,21 @@ Definition zapSubstEnv : Subst -> Subst :=
     Mk_Subst in_scope Core.emptyVarEnv Core.emptyVarEnv Core.emptyVarEnv.
 
 Definition substUnfolding : Subst -> Core.Unfolding -> Core.Unfolding :=
-  fun s u => u.
+  fun arg_0__ arg_1__ => match arg_0__, arg_1__ with | _, unf => unf end.
 
-Axiom substTyVarBndr : Subst -> Core.TyVar -> (Subst * Core.TyVar)%type.
-
-Axiom substTy : Subst -> AxiomatizedTypes.Type_ -> AxiomatizedTypes.Type_.
+Definition substTyVarBndr : Subst -> Core.TyVar -> (Subst * Core.TyVar)%type :=
+  fun arg_0__ arg_1__ =>
+    match arg_0__, arg_1__ with
+    | Mk_Subst in_scope id_env tv_env cv_env, tv =>
+        let 'pair (Core.Mk_TCvSubst in_scope' tv_env' cv_env') tv' :=
+          (@Core.substTyVarBndr tt (Core.Mk_TCvSubst in_scope tv_env cv_env)) tv in
+        pair (Mk_Subst in_scope' id_env tv_env' cv_env') tv'
+    end.
 
 Axiom substSpec : Subst -> Core.Id -> Core.RuleInfo -> Core.RuleInfo.
 
 Definition substInScope : Subst -> Core.InScopeSet :=
   fun '(Mk_Subst in_scope _ _ _) => in_scope.
-
-Definition substIdType : Subst -> Core.Id -> Core.Id :=
-  fun arg_0__ arg_1__ =>
-    match arg_0__, arg_1__ with
-    | (Mk_Subst _ _ tv_env cv_env as subst), id =>
-        let old_ty := Id.idType id in
-        if orb (andb (Core.isEmptyVarEnv tv_env) (Core.isEmptyVarEnv cv_env))
-               (Core.noFreeVarsOfType old_ty) : bool
-        then id else
-        Id.setIdType id (substTy subst old_ty)
-    end.
 
 Definition substIdInfo
    : Subst -> Core.Id -> Core.IdInfo -> option Core.IdInfo :=
@@ -89,46 +84,14 @@ Definition substIdInfo
     Some (Core.setUnfoldingInfo (Core.setRuleInfo info (substSpec subst new_id
                                                    old_rules)) (substUnfolding subst old_unf)).
 
-Definition substIdBndr
-   : String -> Subst -> Subst -> Core.Id -> (Subst * Core.Id)%type :=
-  fun arg_0__ arg_1__ arg_2__ arg_3__ =>
-    match arg_0__, arg_1__, arg_2__, arg_3__ with
-    | _doc, rec_subst, (Mk_Subst in_scope env tvs cvs as subst), old_id =>
-        let old_ty := Id.idType old_id in
-        let no_type_change :=
-          orb (andb (Core.isEmptyVarEnv tvs) (Core.isEmptyVarEnv cvs)) true in
-        let id1 := Core.uniqAway in_scope old_id in
-        let id2 :=
-          if no_type_change : bool then id1 else
-          Id.setIdType id1 (substTy subst old_ty) in
-        let mb_new_info := substIdInfo rec_subst id2 ((@Core.idInfo tt) id2) in
-        let new_id := Id.maybeModifyIdInfo mb_new_info id2 in
-        let no_change := id1 == old_id in
-        let new_env :=
-          if no_change : bool then Core.delVarEnv env old_id else
-          Core.extendVarEnv env old_id (Core.Mk_Var new_id) in
-        pair (Mk_Subst (Core.extendInScopeSet in_scope new_id) new_env tvs cvs) new_id
+Definition substCoVarBndr : Subst -> Core.TyVar -> (Subst * Core.TyVar)%type :=
+  fun arg_0__ arg_1__ =>
+    match arg_0__, arg_1__ with
+    | Mk_Subst in_scope id_env tv_env cv_env, cv =>
+        let 'pair (Core.Mk_TCvSubst in_scope' tv_env' cv_env') cv' :=
+          Core.substCoVarBndr (Core.Mk_TCvSubst in_scope tv_env cv_env) cv in
+        pair (Mk_Subst in_scope' id_env tv_env' cv_env') cv'
     end.
-
-Definition substRecBndrs
-   : Subst -> list Core.Id -> (Subst * list Core.Id)%type :=
-  fun subst bndrs =>
-    let 'pair new_subst new_bndrs := mapAccumL (substIdBndr (Datatypes.id
-                                                             (GHC.Base.hs_string__ "rec-bndr")) (GHC.Err.error
-                                                             Panic.someSDoc)) subst bndrs in
-    pair new_subst new_bndrs.
-
-Axiom substCoVarBndr : Subst -> Core.TyVar -> (Subst * Core.TyVar)%type.
-
-Axiom substCo : Subst -> AxiomatizedTypes.Coercion -> AxiomatizedTypes.Coercion.
-
-Definition substBndr : Subst -> Core.Var -> (Subst * Core.Var)%type :=
-  fun subst bndr =>
-    substIdBndr (Datatypes.id (GHC.Base.hs_string__ "var-bndr")) subst subst bndr.
-
-Definition substBndrs
-   : Subst -> list Core.Var -> (Subst * list Core.Var)%type :=
-  fun subst bndrs => mapAccumL substBndr subst bndrs.
 
 Definition setInScope : Subst -> Core.InScopeSet -> Subst :=
   fun arg_0__ arg_1__ =>
@@ -169,7 +132,14 @@ Definition mkEmptySubst : Core.InScopeSet -> Subst :=
   fun in_scope =>
     Mk_Subst in_scope Core.emptyVarEnv Core.emptyVarEnv Core.emptyVarEnv.
 
-Axiom lookupTCvSubst : Subst -> Core.TyVar -> AxiomatizedTypes.Type_.
+Definition lookupTCvSubst : Subst -> Core.TyVar -> AxiomatizedTypes.Type_ :=
+  fun arg_0__ arg_1__ =>
+    match arg_0__, arg_1__ with
+    | Mk_Subst _ _ tvs cvs, v =>
+        if Core.isTyVar v : bool
+        then Maybes.orElse (Core.lookupVarEnv tvs v) (Core.mkTyVarTy v) else
+        Core.mkCoercionTy (Maybes.orElse (Core.lookupVarEnv cvs v) (Core.mkCoVarCo v))
+    end.
 
 Definition lookupIdSubst : String -> Subst -> Core.Id -> Core.CoreExpr :=
   fun arg_0__ arg_1__ arg_2__ =>
@@ -191,6 +161,105 @@ Definition lookupIdSubst : String -> Subst -> Core.Id -> Core.CoreExpr :=
             end
         end
     end.
+
+Definition substDVarSet : Subst -> Core.DVarSet -> Core.DVarSet :=
+  fun subst fvs =>
+    let subst_fv :=
+      fun subst fv acc =>
+        if Core.isId fv : bool
+        then CoreFVs.expr_fvs (lookupIdSubst (Datatypes.id (GHC.Base.hs_string__
+                                                            "substDVarSet")) subst fv) Core.isLocalVar Core.emptyVarSet
+             acc else
+        FV.emptyFV (const true) Core.emptyVarSet acc in
+    Core.mkDVarSet (Data.Tuple.fst (Data.Foldable.foldr (subst_fv subst) (pair nil
+                                                                               Core.emptyVarSet) (Core.dVarSetElems
+                                                         fvs))).
+
+Definition substIdOcc : Subst -> Core.Id -> Core.Id :=
+  fun subst v =>
+    match lookupIdSubst (Datatypes.id (GHC.Base.hs_string__ "substIdOcc")) subst
+            v with
+    | Core.Mk_Var v' => v'
+    | other => Panic.panicStr (GHC.Base.hs_string__ "substIdOcc") (Panic.someSDoc)
+    end.
+
+Definition substTickish
+   : Subst -> Core.Tickish Core.Id -> Core.Tickish Core.Id :=
+  fun arg_0__ arg_1__ =>
+    match arg_0__, arg_1__ with
+    | subst, Core.Breakpoint n ids =>
+        let do_one :=
+          CoreUtils.getIdFromTrivialExpr ∘
+          lookupIdSubst (Datatypes.id (GHC.Base.hs_string__ "subst_tickish")) subst in
+        Core.Breakpoint n (map do_one ids)
+    | _subst, other => other
+    end.
+
+Definition isInScope : Core.Var -> Subst -> bool :=
+  fun arg_0__ arg_1__ =>
+    match arg_0__, arg_1__ with
+    | v, Mk_Subst in_scope _ _ _ => Core.elemInScopeSet v in_scope
+    end.
+
+Definition isEmptySubst : Subst -> bool :=
+  fun '(Mk_Subst _ id_env tv_env cv_env) =>
+    andb (Core.isEmptyVarEnv id_env) (andb (Core.isEmptyVarEnv tv_env)
+                                           (Core.isEmptyVarEnv cv_env)).
+
+Definition substUnfoldingSC : Subst -> Core.Unfolding -> Core.Unfolding :=
+  fun subst unf =>
+    if isEmptySubst subst : bool then unf else
+    substUnfolding subst unf.
+
+Definition getTCvSubst : Subst -> Core.TCvSubst :=
+  fun '(Mk_Subst in_scope _ tenv cenv) => Core.Mk_TCvSubst in_scope tenv cenv.
+
+Definition substCo
+   : Subst -> AxiomatizedTypes.Coercion -> AxiomatizedTypes.Coercion :=
+  fun subst co => (@Core.substCo tt (getTCvSubst subst)) co.
+
+Definition substTy
+   : Subst -> AxiomatizedTypes.Type_ -> AxiomatizedTypes.Type_ :=
+  fun subst ty => Core.substTyUnchecked (getTCvSubst subst) ty.
+
+Definition substIdBndr
+   : String -> Subst -> Subst -> Core.Id -> (Subst * Core.Id)%type :=
+  fun arg_0__ arg_1__ arg_2__ arg_3__ =>
+    match arg_0__, arg_1__, arg_2__, arg_3__ with
+    | _doc, rec_subst, (Mk_Subst in_scope env tvs cvs as subst), old_id =>
+        let old_ty := Id.idType old_id in
+        let no_type_change :=
+          orb (andb (Core.isEmptyVarEnv tvs) (Core.isEmptyVarEnv cvs)) true in
+        let id1 := Core.uniqAway in_scope old_id in
+        let id2 :=
+          if no_type_change : bool then id1 else
+          Id.setIdType id1 (substTy subst old_ty) in
+        let mb_new_info := substIdInfo rec_subst id2 ((@Core.idInfo tt) id2) in
+        let new_id := Id.maybeModifyIdInfo mb_new_info id2 in
+        let no_change := id1 == old_id in
+        let new_env :=
+          if no_change : bool then Core.delVarEnv env old_id else
+          Core.extendVarEnv env old_id (Core.Mk_Var new_id) in
+        pair (Mk_Subst (Core.extendInScopeSet in_scope new_id) new_env tvs cvs) new_id
+    end.
+
+Definition substBndr : Subst -> Core.Var -> (Subst * Core.Var)%type :=
+  fun subst bndr =>
+    if Core.isTyVar bndr : bool then substTyVarBndr subst bndr else
+    if Core.isCoVar bndr : bool then substCoVarBndr subst bndr else
+    substIdBndr (Datatypes.id (GHC.Base.hs_string__ "var-bndr")) subst subst bndr.
+
+Definition substBndrs
+   : Subst -> list Core.Var -> (Subst * list Core.Var)%type :=
+  fun subst bndrs => mapAccumL substBndr subst bndrs.
+
+Definition substRecBndrs
+   : Subst -> list Core.Id -> (Subst * list Core.Id)%type :=
+  fun subst bndrs =>
+    let 'pair new_subst new_bndrs := mapAccumL (substIdBndr (Datatypes.id
+                                                             (GHC.Base.hs_string__ "rec-bndr")) (GHC.Err.error
+                                                             Panic.someSDoc)) subst bndrs in
+    pair new_subst new_bndrs.
 
 Definition substBind : Subst -> Core.CoreBind -> (Subst * Core.CoreBind)%type :=
   fix subst_expr (doc : String) (subst : Subst) (expr : Core.CoreExpr)
@@ -237,37 +306,15 @@ Definition substBind : Subst -> Core.CoreBind -> (Subst * Core.CoreBind)%type :=
                                  pair subst' (Core.Rec (GHC.List.zip bndrs' rhss'))
                              end for substBind.
 
-Definition substDVarSet : Subst -> Core.DVarSet -> Core.DVarSet :=
-  fun subst fvs =>
-    let subst_fv :=
-      fun subst fv acc =>
-        if Core.isId fv : bool
-        then CoreFVs.expr_fvs (lookupIdSubst (Datatypes.id (GHC.Base.hs_string__
-                                                            "substDVarSet")) subst fv) Core.isLocalVar Core.emptyVarSet
-             acc else
-        FV.emptyFV (const true) Core.emptyVarSet acc in
-    Core.mkDVarSet (Data.Tuple.fst (Data.Foldable.foldr (subst_fv subst) (pair nil
-                                                                               Core.emptyVarSet) (Core.dVarSetElems
-                                                         fvs))).
-
-Definition substIdOcc : Subst -> Core.Id -> Core.Id :=
-  fun subst v =>
-    match lookupIdSubst (Datatypes.id (GHC.Base.hs_string__ "substIdOcc")) subst
-            v with
-    | Core.Mk_Var v' => v'
-    | other => Panic.panicStr (GHC.Base.hs_string__ "substIdOcc") (Panic.someSDoc)
-    end.
-
-Definition substTickish
-   : Subst -> Core.Tickish Core.Id -> Core.Tickish Core.Id :=
+Definition substIdType : Subst -> Core.Id -> Core.Id :=
   fun arg_0__ arg_1__ =>
     match arg_0__, arg_1__ with
-    | subst, Core.Breakpoint n ids =>
-        let do_one :=
-          CoreUtils.getIdFromTrivialExpr ∘
-          lookupIdSubst (Datatypes.id (GHC.Base.hs_string__ "subst_tickish")) subst in
-        Core.Breakpoint n (map do_one ids)
-    | _subst, other => other
+    | (Mk_Subst _ _ tv_env cv_env as subst), id =>
+        let old_ty := Id.idType id in
+        if orb (andb (Core.isEmptyVarEnv tv_env) (Core.isEmptyVarEnv cv_env))
+               (Core.noFreeVarsOfType old_ty) : bool
+        then id else
+        Id.setIdType id (substTy subst old_ty)
     end.
 
 Definition subst_expr : String -> Subst -> Core.CoreExpr -> Core.CoreExpr :=
@@ -315,6 +362,24 @@ Definition subst_expr : String -> Subst -> Core.CoreExpr -> Core.CoreExpr :=
                                  pair subst' (Core.Rec (GHC.List.zip bndrs' rhss'))
                              end for subst_expr.
 
+Definition substBindSC
+   : Subst -> Core.CoreBind -> (Subst * Core.CoreBind)%type :=
+  fun subst bind =>
+    if negb (isEmptySubst subst) : bool then substBind subst bind else
+    match bind with
+    | Core.NonRec bndr rhs =>
+        let 'pair subst' bndr' := substBndr subst bndr in
+        pair subst' (Core.NonRec bndr' rhs)
+    | Core.Rec pairs =>
+        let 'pair bndrs rhss := GHC.List.unzip pairs in
+        let 'pair subst' bndrs' := substRecBndrs subst bndrs in
+        let rhss' :=
+          if isEmptySubst subst' : bool then rhss else
+          map (subst_expr (Datatypes.id (GHC.Base.hs_string__ "substBindSC")) subst')
+          rhss in
+        pair subst' (Core.Rec (GHC.List.zip bndrs' rhss'))
+    end.
+
 Definition substExpr : String -> Subst -> Core.CoreExpr -> Core.CoreExpr :=
   fun doc subst orig_expr => subst_expr doc subst orig_expr.
 
@@ -352,47 +417,10 @@ Definition substRulesForImportedIds
         (Panic.someSDoc) in
     map (substRule subst not_needed) rules.
 
-Definition isInScope : Core.Var -> Subst -> bool :=
-  fun arg_0__ arg_1__ =>
-    match arg_0__, arg_1__ with
-    | v, Mk_Subst in_scope _ _ _ => Core.elemInScopeSet v in_scope
-    end.
-
-Definition isEmptySubst : Subst -> bool :=
-  fun '(Mk_Subst _ id_env tv_env cv_env) =>
-    andb (Core.isEmptyVarEnv id_env) (andb (Core.isEmptyVarEnv tv_env)
-                                           (Core.isEmptyVarEnv cv_env)).
-
-Definition substBindSC
-   : Subst -> Core.CoreBind -> (Subst * Core.CoreBind)%type :=
-  fun subst bind =>
-    if negb (isEmptySubst subst) : bool then substBind subst bind else
-    match bind with
-    | Core.NonRec bndr rhs =>
-        let 'pair subst' bndr' := substBndr subst bndr in
-        pair subst' (Core.NonRec bndr' rhs)
-    | Core.Rec pairs =>
-        let 'pair bndrs rhss := GHC.List.unzip pairs in
-        let 'pair subst' bndrs' := substRecBndrs subst bndrs in
-        let rhss' :=
-          if isEmptySubst subst' : bool then rhss else
-          map (subst_expr (Datatypes.id (GHC.Base.hs_string__ "substBindSC")) subst')
-          rhss in
-        pair subst' (Core.Rec (GHC.List.zip bndrs' rhss'))
-    end.
-
 Definition substExprSC : String -> Subst -> Core.CoreExpr -> Core.CoreExpr :=
   fun doc subst orig_expr =>
     if isEmptySubst subst : bool then orig_expr else
     subst_expr doc subst orig_expr.
-
-Definition substUnfoldingSC : Subst -> Core.Unfolding -> Core.Unfolding :=
-  fun subst unf =>
-    if isEmptySubst subst : bool then unf else
-    substUnfolding subst unf.
-
-Definition getTCvSubst : Subst -> Core.TCvSubst :=
-  fun '(Mk_Subst in_scope _ tenv cenv) => Core.Mk_TCvSubst in_scope tenv cenv.
 
 Definition extendTvSubst
    : Subst -> Core.TyVar -> AxiomatizedTypes.Type_ -> Subst :=
@@ -460,13 +488,6 @@ Definition extendIdSubst : Subst -> Core.Id -> Core.CoreExpr -> Subst :=
         else Mk_Subst in_scope (Core.extendVarEnv ids v r) tvs cvs
     end.
 
-Definition extendSubstWithVar : Subst -> Core.Var -> Core.Var -> Subst :=
-  fun subst v1 v2 =>
-    if andb Util.debugIsOn (negb (Core.isId v2)) : bool
-    then (Panic.assertPanic (GHC.Base.hs_string__
-                             "ghc/compiler/coreSyn/CoreSubst.hs") #245)
-    else extendIdSubst subst v1 (Core.Mk_Var v2).
-
 Definition extendCvSubst
    : Subst -> Core.CoVar -> AxiomatizedTypes.Coercion -> Subst :=
   fun arg_0__ arg_1__ arg_2__ =>
@@ -507,6 +528,23 @@ Definition extendSubstList
            | subst, cons (pair var rhs) prs =>
                extendSubstList (extendSubst subst var rhs) prs
            end.
+
+Definition extendSubstWithVar : Subst -> Core.Var -> Core.Var -> Subst :=
+  fun subst v1 v2 =>
+    if Core.isTyVar v1 : bool
+    then if andb Util.debugIsOn (negb (Core.isTyVar v2)) : bool
+         then (Panic.assertPanic (GHC.Base.hs_string__
+                                  "ghc/compiler/coreSyn/CoreSubst.hs") #243)
+         else extendTvSubst subst v1 (Core.mkTyVarTy v2) else
+    if Core.isCoVar v1 : bool
+    then if andb Util.debugIsOn (negb (Core.isCoVar v2)) : bool
+         then (Panic.assertPanic (GHC.Base.hs_string__
+                                  "ghc/compiler/coreSyn/CoreSubst.hs") #244)
+         else extendCvSubst subst v1 (Core.mkCoVarCo v2) else
+    if andb Util.debugIsOn (negb (Core.isId v2)) : bool
+    then (Panic.assertPanic (GHC.Base.hs_string__
+                             "ghc/compiler/coreSyn/CoreSubst.hs") #245)
+    else extendIdSubst subst v1 (Core.Mk_Var v2).
 
 Definition emptySubst : Subst :=
   Mk_Subst Core.emptyInScopeSet Core.emptyVarEnv Core.emptyVarEnv
@@ -551,8 +589,15 @@ Definition clone_id
              new_id
     end.
 
-Axiom cloneTyVarBndr : Subst ->
-                       Core.TyVar -> Unique.Unique -> (Subst * Core.TyVar)%type.
+Definition cloneTyVarBndr
+   : Subst -> Core.TyVar -> Unique.Unique -> (Subst * Core.TyVar)%type :=
+  fun arg_0__ arg_1__ arg_2__ =>
+    match arg_0__, arg_1__, arg_2__ with
+    | Mk_Subst in_scope id_env tv_env cv_env, tv, uniq =>
+        let 'pair (Core.Mk_TCvSubst in_scope' tv_env' cv_env') tv' :=
+          Core.cloneTyVarBndr (Core.Mk_TCvSubst in_scope tv_env cv_env) tv uniq in
+        pair (Mk_Subst in_scope' id_env tv_env' cv_env') tv'
+    end.
 
 Definition cloneRecIdBndrs
    : Subst ->
@@ -609,20 +654,21 @@ Definition addInScopeSet : Subst -> Core.VarSet -> Subst :=
      Core.Lam Core.Let Core.Lit Core.Mk_Coercion Core.Mk_TCvSubst Core.Mk_Type
      Core.Mk_Var Core.NonRec Core.Rec Core.Rule Core.RuleInfo Core.TCvSubst
      Core.Tickish Core.TvSubstEnv Core.TyVar Core.Unfolding Core.Var Core.VarSet
-     Core.dVarSetElems Core.delVarEnv Core.delVarEnvList Core.elemInScopeSet
-     Core.emptyInScopeSet Core.emptyVarEnv Core.emptyVarSet Core.extendInScopeSet
-     Core.extendInScopeSetList Core.extendInScopeSetSet Core.extendVarEnv
-     Core.extendVarEnvList Core.idInfo Core.isCoVar Core.isEmptyRuleInfo
-     Core.isEmptyVarEnv Core.isFragileUnfolding Core.isId Core.isLocalId
-     Core.isLocalVar Core.isNonCoVarId Core.isTyVar Core.lookupInScope
-     Core.lookupVarEnv Core.mkCoVarCo Core.mkDVarSet Core.mkVarEnv
-     Core.noFreeVarsOfType Core.ruleInfo Core.setRuleInfo Core.setUnfoldingInfo
-     Core.setVarUnique Core.unfoldingInfo Core.uniqAway CoreFVs.expr_fvs
-     CoreUtils.getIdFromTrivialExpr Data.Foldable.all Data.Foldable.foldl'
-     Data.Foldable.foldr Data.Tuple.fst Data.Tuple.snd Datatypes.id FV.emptyFV
-     GHC.Err.error GHC.List.unzip GHC.List.zip GHC.Num.fromInteger Id.idType
-     Id.maybeModifyIdInfo Id.setIdType Name.Name Panic.assertPanic Panic.panicStr
-     Panic.someSDoc Panic.warnPprTrace UniqSupply.UniqSupply
-     UniqSupply.uniqFromSupply UniqSupply.uniqsFromSupply Unique.Unique
-     Util.debugIsOn
+     Core.cloneTyVarBndr Core.dVarSetElems Core.delVarEnv Core.delVarEnvList
+     Core.elemInScopeSet Core.emptyInScopeSet Core.emptyVarEnv Core.emptyVarSet
+     Core.extendInScopeSet Core.extendInScopeSetList Core.extendInScopeSetSet
+     Core.extendVarEnv Core.extendVarEnvList Core.idInfo Core.isCoVar
+     Core.isEmptyRuleInfo Core.isEmptyVarEnv Core.isFragileUnfolding Core.isId
+     Core.isLocalId Core.isLocalVar Core.isNonCoVarId Core.isTyVar Core.lookupInScope
+     Core.lookupVarEnv Core.mkCoVarCo Core.mkCoercionTy Core.mkDVarSet Core.mkTyVarTy
+     Core.mkVarEnv Core.noFreeVarsOfType Core.ruleInfo Core.setRuleInfo
+     Core.setUnfoldingInfo Core.setVarUnique Core.substCo Core.substCoVarBndr
+     Core.substTyUnchecked Core.substTyVarBndr Core.unfoldingInfo Core.uniqAway
+     CoreFVs.expr_fvs CoreUtils.getIdFromTrivialExpr Data.Foldable.all
+     Data.Foldable.foldl' Data.Foldable.foldr Data.Tuple.fst Data.Tuple.snd
+     Datatypes.id FV.emptyFV GHC.Err.error GHC.List.unzip GHC.List.zip
+     GHC.Num.fromInteger Id.idType Id.maybeModifyIdInfo Id.setIdType Maybes.orElse
+     Name.Name Panic.assertPanic Panic.panicStr Panic.someSDoc Panic.warnPprTrace
+     UniqSupply.UniqSupply UniqSupply.uniqFromSupply UniqSupply.uniqsFromSupply
+     Unique.Unique Util.debugIsOn
 *)
