examples/ghc/deps/CoreOpt.mk
@@ -1,1 +1,1 @@
-lib/CoreOpt.v: lib/BasicTypes.h2ci lib/Core.h2ci lib/CoreSubst.h2ci
+lib/CoreOpt.v: lib/BasicTypes.h2ci lib/Core.h2ci lib/CoreSubst.h2ci ../../base/Data/Either.h2ci lib/Pair.h2ci
